deallocate_slab WIP

src/Slabs2.fst
@@ -77,56 +77,174 @@ open Slabs
 //  )
 
 open FStar.Mul
+open SteelStarSeqUtils
+open SteelVRefineDep
+module AL = ArrayList
 
 unfold
 let blob = Slabs.blob
-(*
-#push-options "--compat_pre_typed_indexed_effects --z3rlimit 50"
-let deallocate_slab
-  (size_class: sc)
-  //(partial_slabs_ptr empty_slabs_ptr full_slabs_ptr: ref SL.t)
-  //(partial_slabs empty_slabs full_slabs: SL.t)
-  (slab_region: array U8.t{A.length slab_region == U32.v metadata_max * U32.v page_size})
-  (md_bm_region: array U64.t{A.length md_bm_region = U32.v metadata_max * 4})
-  (md_region: array (AL.cell blob){A.length md_region = U32.v metadata_max})
+
+assume val deallocate_slab_aux_empty
   (ptr: array U8.t)
-  (md_count_v: (x:U32.t{U32.v x <= U32.v metadata_max}))
-  : Steel bool
+  (size_class: sc)
+  (slab_region: array U8.t{A.length slab_region = U32.v metadata_max * U32.v page_size})
+  (md_bm_region: array U64.t{A.length md_bm_region = U32.v metadata_max * 4})
+  (md_region: array AL.cell{A.length md_region = U32.v metadata_max})
+  (md_count: ref U32.t)
+  (r1 r2 r3: ref US.t)
+  (md_count_v: U32.t{U32.v md_count_v < U32.v metadata_max})
+  (md_region_lv: G.erased (Seq.lseq AL.status (U32.v md_count_v)))
+  (idx1 idx2 idx3: US.t)
+  (diff: UP.t)
+  : SteelT bool
   (
     A.varray ptr `star`
-    AL.varraylist (A.split_l md_region (u32_to_sz md_count_v)) 0 `star`
-    A.varray (A.split_l slab_region 0sz)
+    vptr md_count `star`
+    vptr r1 `star`
+    vptr r2 `star`
+    vptr r3 `star`
+    right_vprop slab_region md_bm_region md_region md_count_v `star`
+    (AL.varraylist pred1 pred2 pred3
+      (A.split_l md_region (u32_to_sz md_count_v))
+      (US.v idx1) (US.v idx2) (US.v idx3)) `star`
+    starseq
+      #(pos:U32.t{U32.v pos < U32.v md_count_v})
+      #(t size_class)
+      (f size_class slab_region md_bm_region md_count_v md_region_lv)
+      (f_lemma size_class slab_region md_bm_region md_count_v md_region_lv)
+      (SeqUtils.init_u32_refined (U32.v md_count_v))
   )
   (fun b ->
     (if b then emp else A.varray ptr) `star`
-    AL.varraylist (A.split_l md_region (u32_to_sz md_count_v)) 0 `star`
-    A.varray (A.split_l slab_region 0sz)
+    vrefinedep
+      (vptr md_count)
+      (fun x -> U32.v x <= U32.v metadata_max == true)
+      (fun v ->
+         left_vprop size_class slab_region md_bm_region v md_region r1 r2 r3 `star`
+         right_vprop slab_region md_bm_region md_region v)
+  )
+
+assume val deallocate_slab_aux_partial
+  (ptr: array U8.t)
+  (size_class: sc)
+  (slab_region: array U8.t{A.length slab_region = U32.v metadata_max * U32.v page_size})
+  (md_bm_region: array U64.t{A.length md_bm_region = U32.v metadata_max * 4})
+  (md_region: array AL.cell{A.length md_region = U32.v metadata_max})
+  (md_count: ref U32.t)
+  (r1 r2 r3: ref US.t)
+  (md_count_v: U32.t{U32.v md_count_v < U32.v metadata_max})
+  (md_region_lv: G.erased (Seq.lseq AL.status (U32.v md_count_v)))
+  (idx1 idx2 idx3: US.t)
+  (diff: UP.t)
+  : SteelT bool
+  (
+    A.varray ptr `star`
+    vptr md_count `star`
+    vptr r1 `star`
+    vptr r2 `star`
+    vptr r3 `star`
+    right_vprop slab_region md_bm_region md_region md_count_v `star`
+    (AL.varraylist pred1 pred2 pred3
+      (A.split_l md_region (u32_to_sz md_count_v))
+      (US.v idx1) (US.v idx2) (US.v idx3)) `star`
+    starseq
+      #(pos:U32.t{U32.v pos < U32.v md_count_v})
+      #(t size_class)
+      (f size_class slab_region md_bm_region md_count_v md_region_lv)
+      (f_lemma size_class slab_region md_bm_region md_count_v md_region_lv)
+      (SeqUtils.init_u32_refined (U32.v md_count_v))
+  )
+  (fun b ->
+    (if b then emp else A.varray ptr) `star`
+    vrefinedep
+      (vptr md_count)
+      (fun x -> U32.v x <= U32.v metadata_max == true)
+      (fun v ->
+         left_vprop size_class slab_region md_bm_region v md_region r1 r2 r3 `star`
+         right_vprop slab_region md_bm_region md_region v)
+  )
+
+#push-options "--compat_pre_typed_indexed_effects --z3rlimit 50"
+let deallocate_slab'
+  (ptr: array U8.t)
+  (size_class: sc)
+  (slab_region: array U8.t{A.length slab_region = U32.v metadata_max * U32.v page_size})
+  (md_bm_region: array U64.t{A.length md_bm_region = U32.v metadata_max * 4})
+  (md_region: array AL.cell{A.length md_region = U32.v metadata_max})
+  (md_count: ref U32.t)
+  (r1 r2 r3: ref US.t)
+  (md_count_v: U32.t{U32.v md_count_v < U32.v metadata_max})
+  (md_region_lv: G.erased (Seq.lseq AL.status (U32.v md_count_v)))
+  (idx1 idx2 idx3: US.t)
+  (diff: UP.t)
+  : Steel bool
+  (
+    A.varray ptr `star`
+    vptr md_count `star`
+    vptr r1 `star`
+    vptr r2 `star`
+    vptr r3 `star`
+    right_vprop slab_region md_bm_region md_region md_count_v `star`
+    (AL.varraylist pred1 pred2 pred3
+      (A.split_l md_region (u32_to_sz md_count_v))
+      (US.v idx1) (US.v idx2) (US.v idx3)) `star`
+    starseq
+      #(pos:U32.t{U32.v pos < U32.v md_count_v})
+      #(t size_class)
+      (f size_class slab_region md_bm_region md_count_v md_region_lv)
+      (f_lemma size_class slab_region md_bm_region md_count_v md_region_lv)
+      (SeqUtils.init_u32_refined (U32.v md_count_v))
+  )
+  (fun b ->
+    (if b then emp else A.varray ptr) `star`
+    vrefinedep
+      (vptr md_count)
+      (fun x -> U32.v x <= U32.v metadata_max == true)
+      (fun v ->
+         left_vprop size_class slab_region md_bm_region v md_region r1 r2 r3 `star`
+         right_vprop slab_region md_bm_region md_region v)
   )
   (requires fun h0 ->
-    //TODO: FIXME @Aymeric
-    //let s = h0 (AL.varraylist (A.split_l md_region (u32_to_sz md_count_v)) 0) in
-    let diff = A.offset (A.ptr_of ptr) - A.offset (A.ptr_of slab_region) in
-    same_base_array ptr slab_region /\
-    0 <= diff /\
-    UP.fits ((U32.v page_size) * (U32.v metadata_max)) /\
-    diff < (U32.v page_size) * (U32.v metadata_max) /\
-    (U32.v page_size) % (U32.v size_class) = 0 /\
-    U32.v md_count_v <= U32.v metadata_max
-
+    let diff' = A.offset (A.ptr_of ptr) - A.offset (A.ptr_of slab_region) in
+    0 <= diff' /\
+    UP.v diff == diff' /\
+    sel r1 h0 == idx1 /\
+    sel r2 h0 == idx2 /\
+    sel r3 h0 == idx3 /\
+    md_count_v == sel md_count h0
   )
   (ensures fun _ _ _ -> True)
   =
-  let diff = A.ptrdiff ptr (A.split_l slab_region 0sz) in
   let diff_sz = UP.ptrdifft_to_sizet diff in
   assume (US.fits_u32);
   assert_norm (4 < FI.max_int 16);
   let diff_u32 = US.sizet_to_uint32 diff_sz in
-  assert (U32.v diff_u32 == UP.v diff);
+  assume (U32.v diff_u32 == UP.v diff);
   let pos = U32.div diff_u32 page_size in
   // check diff/page_size < md_count
   if U32.lt pos md_count_v then (
-    // get corresponding slab/md pointers
-    let b = AL.read_in_place (A.split_l md_region (u32_to_sz md_count_v)) 0 (u32_to_sz pos) in
+    let status1 = 0ul in
+    if (U32.eq status1 2ul) then (
+      sladmit ();
+      return false
+    ) else if (U32.eq status1 1ul) then (
+      let b = deallocate_slab_aux_partial ptr size_class
+        slab_region md_bm_region md_region md_count r1 r2 r3
+        md_count_v md_region_lv idx1 idx2 idx3 diff in
+      return b
+    ) else (
+      let b = deallocate_slab_aux_empty ptr size_class
+        slab_region md_bm_region md_region md_count r1 r2 r3
+        md_count_v md_region_lv idx1 idx2 idx3 diff in
+      return b
+    )
+  ) else (
+    sladmit ();
+    return false
+  )
+
+(*)
+
     // refinement: Steel issue, does not work as logical precond
     assume (snd b == slab_array slab_region pos);
     // ArrayList predicate + unpacking/packing support 1/2
@@ -152,4 +270,3 @@ let deallocate_slab
   ) else (
     return false
   )
-*)
